docs/manual/tutorial/index.md
@@ -9,11 +9,11 @@ programs using the hax toolchain. hax is a tool that translates Rust
 programs to various formal programming languages.
 
 The formal programming languages we target are called *backends*. Some
-of them, e.g. [F\*](https://fstar-lang.org/) or
+of them, e.g. [F\*](https://fstar-lang.org/), [Lean](https://lean-lang.org/) or
 [Coq](https://coq.inria.fr/), are general purpose formal programming
 languages. Others are specialized tools:
 [ProVerif](https://bblanche.gitlabpages.inria.fr/proverif/) is
 dedicated to proving properties about protocols.
 
-This tutorial focuses on proving properties with the
-[F\* programming language](https://fstar-lang.org/).
+This tutorial focuses on proving properties with
+[F\*](https://fstar-lang.org/) or [Lean](https://lean-lang.org/).
